Iris/Iris/ProofMode/InstancesLater.lean
@@ -318,6 +318,42 @@ instance (priority := default - 10) elimModal_timeless [BI PROP] p (P P' Q : PRO
   ElimModal True p p P P' Q Q where
   elim_modal _ := ((sep_mono ((intuitionisticallyIf_mono into_except0).trans except0_intuitionisticallyIf) except0_intro).trans $ except0_sep.2.trans (except0_mono wand_elim_right)).trans is_except0
 
+/-- AddModal -/
+@[rocq_alias add_modal_later_except_0]
+instance (priority := default + 10) addModal_later_except_0 [BI PROP] (P Q : PROP) [h : Timeless P] :
+    AddModal iprop(▷ P) P iprop(◇ Q) where
+  add_modal := calc
+    _ ⊢ ◇ P ∗ (P -∗ ◇ Q)   := sep_mono_left h.timeless
+    _ ⊢ ◇ (P ∗ (P -∗ ◇ Q)) := except0_frame_right
+    _ ⊢ ◇ (◇ Q)            := except0_mono wand_elim_right
+    _ ⊢ ◇ Q                 := except0_idem.mp
+
+@[rocq_alias add_modal_later]
+instance (priority := default + 10) addModal_later [BI PROP] (P Q : PROP) [h : Timeless P] :
+    AddModal iprop(▷ P) P iprop(▷ Q) where
+  add_modal := calc
+    _ ⊢ ◇ P ∗ (P -∗ ▷ Q)   := sep_mono_left h.timeless
+    _ ⊢ ◇ (P ∗ (P -∗ ▷ Q)) := except0_frame_right
+    _ ⊢ ◇ (▷ Q)            := except0_mono wand_elim_right
+    _ ⊢ ▷ Q                 := except0_later
+
+@[rocq_alias add_modal_except_0]
+instance addModal_except_0 [BI PROP] (P Q : PROP) :
+    AddModal iprop(◇ P) P iprop(◇ Q) where
+  add_modal :=
+    calc
+    _ ⊢ ◇ (P ∗ (P -∗ ◇ Q)) := except0_frame_right
+    _ ⊢ ◇ (◇ Q)            := except0_mono wand_elim_right
+    _ ⊢ ◇ Q                 := except0_idem.mp
+
+@[rocq_alias add_modal_except_0_later]
+instance addModal_except_0_later [BI PROP] (P Q : PROP) :
+    AddModal iprop(◇ P) P iprop(▷ Q) where
+  add_modal := calc
+    _ ⊢ ◇ (P ∗ (P -∗ ▷ Q)) := except0_frame_right
+    _ ⊢ ◇ (▷ Q)            := except0_mono wand_elim_right
+    _ ⊢ ▷ Q                 := except0_later
+
 /-- IntoLaterN -/
 @[rocq_alias maybe_into_laterN_default]
 instance (priority := low) intoLaterN_default [BI PROP] only_head n (P : PROP) :
@@ -369,6 +405,7 @@ instance intoLaterN_or [BI PROP] n (P1 P2 Q1 Q2 : PROP)
     [h1 : IntoLaterN false n P1 Q1] [h2 : IntoLaterN false n P2 Q2] :
     IntoLaterN false n iprop(P1 ∨ P2) iprop(Q1 ∨ Q2) where
   into_laterN := (or_mono h1.1 h2.1).trans (laterN_or n).2
+
 
 @[rocq_alias into_later_affinely]
 instance intoLaterN_affinely [BI PROP] n (P Q : PROP)
